finished splitting. also deleted some obsolete stuff. the new proof checks.

monadproofs/proofs/execute_transaction_spec.v
@@ -5,6 +5,12 @@ Require Import stdpp.gmap.
 Require Import monad.proofs.misc.
 Require Import monad.proofs.libspecs.
 Require Import monad.proofs.evmopsem.
+Import linearity.
+Require Import bedrock.auto.invariants.
+Require Import bedrock.auto.cpp.proof.
+
+Require Import bedrock.auto.cpp.tactics4.
+
 
 Import cQp_compat.
 
@@ -16,9 +22,7 @@ Import cancelable_invariants.
 Module BlockState. Section with_Sigma.
   Context `{Sigma:cpp_logic} {CU: genv} {hh: HasOwn mpredI fracR}. (* some standard assumptions about the c++ logic *)
 
-   (* this comes from the iris separation logic library *)
-
-   (* this comes from the iris separation logic library *)
+   (*TODO:  delete? this comes from the iris separation logic library *)
   Definition cinvq (g : gname) (q : Qp) (P : mpred) := cinv_own g q ** cinv nroot (* FIX? *) g P.
   
 
@@ -61,34 +65,12 @@ Open Scope cpp_name.
 Section with_Sigma.
   Context `{Sigma:cpp_logic} {CU: genv} {hh: HasOwn mpredI fracR}. (* some standard assumptions about the c++ logic *)
 
-    (* set_value() passes the resource/assertion P to the one calling get_future->wait()*)
-  Definition PromiseR (g: gname) (P: mpred) : Rep. Proof. Admitted.
-  Definition PromiseProducerR (g: gname) (P: mpred) : Rep. Proof. Admitted.
-  Definition PromiseConsumerR (g: gname) (P: mpred) : Rep. Proof. Admitted.
-  Definition PromiseUnusableR: Rep. Proof. Admitted.
-
-  Lemma sharePromise g P:  PromiseR g P -|- PromiseProducerR g P **  PromiseConsumerR g P.
-  Proof. Admitted.
    
   (* defines how [c] is represented in memory as an object of class Chain. this predicate asserts [q] ownership of the object, assuming it can be shared across multiple threads  *)
   Definition ChainR (q: Qp) (c: Chain): Rep. Proof. Admitted.
-
-  (* defines how [c] is represented in memory as an object of class Chain *)
-  Definition PriorityPoolR (q: Qp) (c: PriorityPool): Rep. Proof. Admitted.
-
-  Definition VectorRbase (cppType: type) (q:Qp) (base: ptr) (size: N): Rep.
-  Proof using.
-    (*Exists cap, 
-       _field "base" |-> ptrR q base
-       ** _field "size" |-> intR q size
-       ** _field "capacity" |-> intR q cap *)
-  Admitted.
-  
- Definition VectorR {ElemType} (cppType: type) (elemRep: ElemType -> Rep) (q:Qp) (lt:list ElemType): Rep :=
-   Exists (base: ptr), VectorRbase cppType q base (lengthN lt)
-       ** pureR (base |-> arrayR cppType elemRep lt).
  
-  Definition TransactionR (q:Qp) (t: Transaction) : Rep. Proof using. Admitted.
+  Definition TransactionR (q:Qp) (tq: Transaction) : Rep. Proof using. Admitted.
+  #[global] Instance learnTrRbase: LearnEq2 TransactionR:= ltac:(solve_learnable).
  
   Definition BlockR (q: Qp) (c: Block): Rep :=
     _field ``::monad::Block::transactions`` |-> VectorR (Tnamed ``::monad::Transaction``) (fun t => TransactionR q t) q (transactions c)
@@ -98,23 +80,6 @@ Section with_Sigma.
   Definition ReceiptR (t: TransactionResult): Rep. Admitted.
   
   Definition valOfRev (r : Revision) : val := Vint 0. (* TODO: fix *)
-
-(*  
-  Definition execute_block_spec : WpSpec mpredI val val :=
-    \arg{chainp :ptr} "chain" (Vref chainp)
-    \prepost{(qchain:Qp) (chain: Chain)} chainp |-> ChainR qchain chain
-    \arg "rev" (valOfRev Shanghai)
-    \arg{blockp: ptr} "block" (Vref blockp)
-    \prepost{(block: Block)} blockp |-> BlockR 1 block (* is this modified? if so, fix this line, else make it const in C++ code? *)
-    \arg{block_statep: ptr} "block_state" (Vref block_statep)
-    \prepost{(preBlockState: StateOfAccounts) (gl: BlockState.glocs)}
-      block_statep |-> BlockState.Rc block preBlockState 1 gl
-    \arg{block_hash_bufferp: ptr} "block_hash_buffer" (Vref block_hash_bufferp)
-    \arg{priority_poolp: ptr} "priority_pool" (Vref priority_poolp)
-    \prepost{priority_pool: PriorityPool} priority_poolp |-> PriorityPoolR 1 priority_pool
-    \post storedAtGhostLoc (2/3)%Q (BlockState.commitedIndexLoc gl) (length (transactions block)).
-
- *)
   
   Definition execute_block_simpler : WpSpec mpredI val val :=
     \arg{chainp :ptr} "chain" (Vref chainp)
@@ -134,16 +99,9 @@ Section with_Sigma.
       ** block_statep |-> BlockState.R block preBlockState actual_final_state.
 
 Import namemap.
-Locate symbols.
 Import translation_unit.
-Check (NM.elements module.(symbols)).
 Require Import List.
-Locate BS.String.
 Import bytestring_core.
-Definition xx:=
-  (bytestring_core.BS.String "s"
-                                 (bytestring_core.BS.String "t"
-                                    (bytestring_core.BS.String "d" bytestring_core.BS.EmptyString))).
 Require Import bedrock.auto.cpp.
 Require Import bedrock.auto.cpp.specs.
 
@@ -154,85 +112,12 @@ Require Import bedrock.auto.cpp.specs.
 
  *)
 
-Require Import bedrock.auto.cpp.tactics4.
-
-Ltac slauto := go; try name_locals; tryif progress(try (ego; eagerUnifyU; go; fail); try (apply False_rect; try contradiction; try congruence; try nia; fail); try autorewrite with syntactic equiv iff slbwd in *; try rewrite left_id)
-  then slauto  else idtac.
 
 Context  {MODd : exb.module ⊧ CU}.
-(* Node::Node(Node*,int) *)
-  Definition promise_constructor_spec (this:ptr) :WpSpec mpredI val val :=
-    \pre{P:mpred} emp
-    \post Exists g:gname, this |->  PromiseR g P.
-  
-  cpp.spec "boost::fibers::promise<void>::set_value()"  as set_value with
-     (fun (this:ptr) =>
-    \pre{(P:mpred) (g:gname)} this |-> PromiseProducerR g P
-    \pre P
-    \post emp).
-
   cpp.spec (Ninst
    "monad::execute_block(const monad::Chain&, monad::Block&, monad::BlockState&, const monad::BlockHashBuffer&, monad::fiber::PriorityPool&)"
    [Avalue (Eint 11 "enum evmc_revision")]) as exbb_spec with (execute_block_simpler).
 
-  cpp.spec
-    "std::vector<monad::Transaction, std::allocator<monad::Transaction>>::size() const"
-    as tvector_spec with
-      (fun (this:ptr) =>
-         \prepost{q base size} this |-> VectorRbase (Tnamed ``::monad::Transaction``)  q base size
-         \post[Vn size] (emp:mpred)
-      ).
-  Print lt.
-
-
-  Definition optionAddressR (q:Qp) (oaddr: option evm.address): Rep. Proof. Admitted.
-
-Definition parrayR  {T:Type} ty (Rs : nat -> T -> Rep) (l: list T) : Rep :=
-  .[ ty ! length l ] |-> validR ** [| is_Some (size_of _ ty) |] **
-  (* ^ both of these are only relevant for empty arrays, otherwise, they are implied by the
-     following conjunct *)
-     [∗ list] i ↦ li ∈ l, .[ ty ! Z.of_nat i ] |-> (type_ptrR ty ** Rs i li).
-
-
-  Lemma arrR_cons0 ty R Rs :
-    arrR ty (R :: Rs) -|- type_ptrR ty ** (.[ ty ! 0 ] |-> R) ** .[ ty ! 1 ] |-> arrR ty Rs.
-  Proof.
-    rewrite arrR_eq/arrR_def /= !_offsetR_sep !_offsetR_only_provable.
-    apply: (observe_both (is_Some (size_of _ ty))) => Hsz.
-    rewrite !_offsetR_sub_0; auto.
-    rewrite _offsetR_big_sepL -assoc.
-    rewrite _offsetR_succ_sub Nat2Z.inj_succ;
-      setoid_rewrite _offsetR_succ_sub; setoid_rewrite Nat2Z.inj_succ.
-    iSplit; [ iIntros "(? & ? & ? & ? & ?)" | iIntros "(? & ? & ? & ? & ?)"]; iFrame.
-  Qed.
-
-  Lemma arrayR_cons0 {T} ty (R:T->Rep) x xs :
-    arrayR ty R (x :: xs) -|- type_ptrR ty ** (.[ ty ! 0 ] |-> R x) ** .[ ty ! 1 ] |-> arrayR ty R xs.
-  Proof. rewrite arrayR_eq. unfold arrayR_def. exact: arrR_cons0. Qed.
-
-  Definition offsetR_only_fwd := ([BWD->] _offsetR_only_provable).
-  Hint Resolve offsetR_only_fwd: br_opacity.
-  Lemma parrayR_cons {T:Type} ty (R : nat -> T -> Rep) (x:T) (xs: list T) :
-    parrayR ty R (x :: xs) -|- type_ptrR ty ** (.[ ty ! 0 ] |-> (R 0 x)) ** .[ ty ! 1 ] |-> parrayR ty (fun n => R (S n)) xs.
-  Proof using.
-    unfold parrayR.
-    apply: (observe_both (is_Some (size_of _ ty))) => Hsz.
-    repeat rewrite !_offsetR_sub_0; auto.
-    repeat rewrite _offsetR_sep.
-    repeat rewrite _offsetR_big_sepL.
-    repeat rewrite _offsetR_succ_sub.
-    repeat setoid_rewrite  _offsetR_succ_sub.
-    simpl.
-    repeat rewrite Nat2Z.inj_succ.
-    repeat rewrite !_offsetR_sub_0; auto.
-    setoid_rewrite Nat2Z.inj_succ.
-    iSplit; work.
-  Qed.
-  Opaque parrayR.
-  Hypothesis sender: Transaction -> evm.address.
-
-
-  Hint Rewrite offset_ptr_sub_0 using (auto; apply has_size; exact _): syntactic.
 
   cpp.spec 
   "monad::reset_promises(unsigned long)" as reset_promises
@@ -274,580 +159,20 @@ cpp.spec
     \arg{trp: ptr} "tr" (Vref trp)
     \prepost{qt (tr: Transaction)} trp |-> TransactionR qt tr
     \post{retp} [Vptr retp] retp |-> optionAddressR 1 (Some (sender tr))).
-    (*
-  cpp.spec
-    "std::vector<monad::Transaction, std::allocator<monad::Transaction>>::size() const"
-    as csector_spec with
-      (fun (this:ptr) =>
-         \prepost{q ts} this |-> VectorR (Tnamed ``::monad::Transaction``) TransactionR q (ts)
-         \post[Vn (lengthN ts)] (emp:mpred)
-      ).
-*)
-  Definition lamName :name :=
-    "monad::compute_senders(std::optional<evmc::address>*, const monad::Block&, monad::fiber::PriorityPool&)::@0".
 
-  Definition lamBody :option GlobDecl := Eval vm_compute in
-    NM.map_lookup lamName (types module).
-
-(*  Definition forkEntry : list (name * ObjValue) := *)
-
-    Print atomic_name_.
-  Fixpoint isFunctionNamed2 (fname: ident) (n:name): bool :=
-    match n with
-    | Nglobal  (Nfunction _ (Nf i) _) => bool_decide (i=fname)
-    | Ninst nm _ => isFunctionNamed2 fname nm
-    | Nscoped _ (Nfunction _ (Nf i) _) => bool_decide (i=fname)
-    | _ => false
-    end.
-
-  Fixpoint containsDep (n:name): bool :=
-    match n with
-    | Ndependent _ => true
-    | Nglobal  (Nfunction _ (Nf i) _) => false
-    | Ninst nm _ => containsDep nm
-    | Nscoped nm (Nfunction _ (Nf i) _) => containsDep nm
-    | _ => false
-    end.
-  
-  Definition findBodyOfFnNamed2 module filter :=
-    List.filter (fun p => let '(nm, body):=p in filter nm) (NM.elements (symbols module)).
-
-
-  Definition firstEntryName (l :list (name * ObjValue)) :=
-    (List.nth 0 (map fst l) (Nunsupported "impossible")).
-  
-  Definition fork_task_namei:= Eval vm_compute in (firstEntryName (findBodyOfFnNamed2 exb.module (isFunctionNamed2 "fork_task"))).
-
-  Definition basee3 (n:name) :=
-    match n with
-    | Ninst (Nscoped (Nglobal (Nid scopename)) _) targs => scopename
-    | _ => ""%pstring
-    end.
-
-  Definition all_but_last {T:Type} (l: list T):= take (length l -1)%nat l. 
-  Definition fork_task_nameg (taskLamStructTy: core.name) :=
-    match fork_task_namei with
-    | Ninst (Nscoped (Nglobal (Nid scopename)) (Nfunction q (Nf base) argTypes)) templateArgs =>
-        let argTypes' := all_but_last argTypes ++  [Tref (Tqualified QC (Tnamed taskLamStructTy))] in
-        Ninst (Nscoped (Nglobal (Nid scopename)) (Nfunction q (Nf base) argTypes')) [Atype (Tnamed taskLamStructTy)]
-    | _ => Nunsupported "no match"
-    end.
-
-
-  Lemma fork_task_name_inst: exists ty, fork_task_nameg ty = fork_task_namei.
-  Proof using.
-    unfold fork_task_nameg. unfold fork_task_namei.
-    eexists. reflexivity.
-  Qed.
-
-  Definition taskOpName : atomic_name := Nfunction function_qualifiers.Nc (Nop OOCall) [].
-  
-  Definition taskOpSpec (lamStructName: core.name) (objOwnership: Rep) (taskPre: mpred):=
-    specify {| info_name :=  (Nscoped lamStructName taskOpName) ;
-              info_type := tMethod lamStructName QC "void" [] |}
-      (fun (this:ptr) =>
-         \prepost this |-> objOwnership
-         \pre taskPre
-         \post emp).
-  
-  Definition forkTaskSpec (lamStructName: core.name) : WpSpec mpredI val val :=
-    \arg{priority_poolp: ptr} "priority_pool" (Vref priority_poolp)
-    \prepost{priority_pool: PriorityPool} priority_poolp |-> PriorityPoolR 1 priority_pool
-    \arg{priority} "i" (Vint priority)  
-    \arg{task:ptr} "func" (Vref task)
-    \pre{objOwnership taskPre} taskOpSpec lamStructName objOwnership taskPre
-    \prepost task |-> objOwnership
-    \pre taskPre
-    \post emp.
-  
-  Lemma learnVUnsafe e t (r:e->Rep): LearnEq2 (VectorR t r).
-  Proof. solve_learnable. Qed.
-  Lemma learnVUnsafe2 e t: LearnEq3 (@VectorR e t).
-  Proof. solve_learnable. Qed.
-
-  Existing Instance learnVUnsafe2.
-  Lemma learnArrUnsafe e t: LearnEq2 (@arrayR _ _ _ e _ t).
-  Proof. solve_learnable. Qed.
-  Lemma learnpArrUnsafe e t: LearnEq2 (@parrayR e t).
-  Proof. solve_learnable. Qed.
-  
-  Existing Instance learnArrUnsafe.
-  Existing Instance learnpArrUnsafe.
-  Hint Opaque parrayR: br_opacity.
-  
-  (* not in use anymore *)
-  Lemma promiseArrDecompose (p:ptr) prIds ltr promiseRes:
-    p |-> parrayR "boost::fibers::promise<void>"
-            (λ (i : nat) (t : Transaction),
-               PromiseR (prIds i) (promiseRes i t))
-            ltr
-   -|- (valid_ptr (p .[ "boost::fibers::promise<void>" ! length ltr ])) **
-      [| is_Some (glob_def CU "boost::fibers::promise<void>" ≫= GlobDecl_size_of) |]         **
-      ([∗ list] k↦_ ∈ ltr, □ (type_ptr "boost::fibers::promise<void>" (p .[ "boost::fibers::promise<void>" ! k ]))) ∗
-      ([∗ list] k↦t ∈ ltr, p .[ "boost::fibers::promise<void>" ! k ] |-> PromiseProducerR (prIds k) (promiseRes k t)) ∗
-      ([∗ list] k↦t ∈ ltr, p .[ "boost::fibers::promise<void>" ! k ] |-> PromiseConsumerR (prIds k) (promiseRes k t)).
-  Proof using.
-    Transparent parrayR. unfold parrayR.
-    iSplit.
-    - 
-      go.
-       setoid_rewrite sharePromise.
-       go.
-       repeat rewrite _at_big_sepL.
-       erewrite big_sepL_mono.
-       2:{
-         intros.
-         go.
-       }
-       simpl. 
-       repeat setoid_rewrite big_sepL_sep.
-       go.
-       setoid_rewrite (@right_id _ _ ((True)%I:mpred));[go | go; rewrite bi.and_elim_l; go].
-    - go.
-       setoid_rewrite sharePromise.
-       go.
-       repeat rewrite _at_big_sepL.
-       hideLhs.
-       erewrite big_sepL_proper .
-       2:{
-         intros.
-         iSplitL.
-         go.
-         simpl.
-         go.
-       }
-       simpl.
-       unhideAllFromWork.
-       repeat setoid_rewrite big_sepL_sep.
-       go.
-       rewrite big_sepL_emp. go.
-       setoid_rewrite (@right_id _ _ ((True)%I:mpred)); go. 
-  Qed.
-Lemma cancelLstar {PROP:bi} {T} l (va vb : T -> PROP):
-  (forall id, id ∈ l -> va id |-- vb id) ->
-  ([∗ list] id ∈ l, va id) |-- ([∗ list] id ∈ l,vb id).
-Proof using.
-  intros He.
-  apply big_sepL_mono.
-  intros.
-  apply He.
-  eapply elem_of_list_lookup_2; eauto.
-Qed.
-
-  Lemma promiseArrDecompose2 (p:ptr) prIds ltr promiseRes:
-    p |-> parrayR "boost::fibers::promise<void>"
-            (λ (i : nat) (t : Transaction),
-               PromiseR (prIds i) (promiseRes i t))
-            ltr
-   -|- (valid_ptr (p .[ "boost::fibers::promise<void>" ! length ltr ])) **
-      [| is_Some (glob_def CU "boost::fibers::promise<void>" ≫= GlobDecl_size_of) |]         **
-      (□ ([∗ list] k↦_ ∈ ltr,  (type_ptr "boost::fibers::promise<void>" (p .[ "boost::fibers::promise<void>" ! k ])))) ∗
-      ([∗ list] k↦t ∈ ltr, p .[ "boost::fibers::promise<void>" ! k ] |-> PromiseProducerR (prIds k) (promiseRes k t)) ∗
-      ([∗ list] k↦t ∈ ltr, p .[ "boost::fibers::promise<void>" ! k ] |-> PromiseConsumerR (prIds k) (promiseRes k t)).
-  Proof using.
-    rewrite promiseArrDecompose.
-    iSplit.
-    - go.
-      icancel @big_sepL_mono; go.
-    -  go.
-       hideLhs.
-       rewrite big_sepL_proper; try go.
-       2:{ intros. iSplit. 2:{go.  evartacs.maximallyInstantiateLhsEvar. }  go. }
-       simpl.
-       unhideAllFromWork.
-       go.
-     Qed.
-  Opaque parrayR.
 
 cpp.spec (fork_task_nameg "monad::compute_senders(const monad::Block&, monad::fiber::PriorityPool&)::@0") as fork_task with (forkTaskSpec "monad::compute_senders(const monad::Block&, monad::fiber::PriorityPool&)::@0").
-  
-#[global] Instance learnPpool : LearnEq2 PriorityPoolR := ltac:(solve_learnable).
-    Require Import bedrock.auto.invariants.
-
-    (* TODO: move out of section *)
-    Ltac aggregateRepPieces base :=
-      repeat rewrite <- (_at_offsetR base);
-      repeat (IPM.perm_left ltac:(fun L n =>
-                            lazymatch L with
-                            | base |-> _ => iRevert n
-                            end
-        ));
-      repeat rewrite bi.wand_curry;
-      repeat rewrite <- _at_sep;
-      match goal with
-        [ |-environments.envs_entails _ (base |-> ?R -* _)] =>
-          iIntrosDestructs;
-          iExists R
-      end.
-
-
-  Definition vector_opg (cppType: type) (this:ptr): WpSpec mpredI val val :=
-    \arg{index} "index" (Vn index)
-    \prepost{qb base size} this |-> VectorRbase cppType qb base size
-    \require (index<size)%Z
-    \post [Vref (base ,, .[cppType!index])] emp.
-
 
     (* todo: generalize over the template arg *)
 cpp.spec 
   "std::vector<monad::Transaction, std::allocator<monad::Transaction>>::operator[](unsigned long) const" as vector_op_monad with (vector_opg "monad::Transaction").
 
-Opaque VectorR.
-       #[global] Instance learnVectorRbase: LearnEq4 VectorRbase:= ltac:(solve_learnable).
-
-       (* TODO: generalize over template arg *)
-  cpp.spec "std::optional<evmc::address>::operator=(std::optional<evmc::address>&&)" as opt_move_assign with
-    (fun (this:ptr) =>
-       \arg{other} "other" (Vptr other)
-       \pre{q oaddr} other |-> optionAddressR q oaddr
-       \pre{prev} this |-> optionAddressR 1 prev
-       \post [Vptr this] this |-> optionAddressR 1 oaddr **  other |-> optionAddressR q None
-    ).
-           
-       Set Nested Proofs Allowed.
-       cpp.spec (Nscoped "std::optional<evmc::address>" (Nfunction function_qualifiers.N Ndtor [])) as destrop with
-           (fun (this:ptr) =>
-              \pre{oa} this |-> optionAddressR 1 oa
-              \post emp
-           ).
-       
-       #[global] Instance learnTrRbase: LearnEq2 TransactionR:= ltac:(solve_learnable).
-       Import Verbose.
-       #[global] Instance learnTrRbase2: LearnEq2 optionAddressR:= ltac:(solve_learnable).
-       #[global] Instance : LearnEq2 PromiseR := ltac:(solve_learnable).
-       #[global] Instance : LearnEq2 PromiseProducerR:= ltac:(solve_learnable).
-
-  Lemma parrayR_sep {V} ty xs  : forall (A B : nat -> V -> Rep),
-    parrayR ty (fun i v => A i v ** B i v) xs -|-
-    parrayR ty (fun i v => A i v) xs **
-    parrayR ty (fun i v=> B i v) xs.
-  Proof.
-    elim: xs => [|x xs IH] /=; intros.
-    Transparent parrayR.
-    - unfold parrayR. simpl. iSplit; go.
-    - repeat rewrite parrayR_cons.  simpl.
-      rewrite {}IH. repeat rewrite _offsetR_sep.
-    all: iSplit; work.
-  Qed.
-
-  #[global] Instance parrayR_proper X ty:
-    Proper ((pointwise_relation nat (pointwise_relation X (≡))) ==> (=) ==> (≡)) (parrayR ty).
-  Proof.
-    unfold parrayR.
-    intros f g Hf xs y ?. subst. f_equiv.
-    f_equiv.
-    f_equiv.
-    hnf.
-    intros. hnf. intros.
-    hnf in Hf.
-    rewrite Hf.
-    reflexivity.
-  Qed.
-
-  #[global] Instance arrayR_mono X ty:
-    Proper (pointwise_relation nat (pointwise_relation X (⊢)) ==> (=) ==> (⊢)) (parrayR ty).
-  Proof.
-    unfold parrayR.
-    intros f g Hf xs y ?. subst. f_equiv.
-    f_equiv.
-    f_equiv.
-    hnf.
-    intros. hnf. intros.
-    hnf in Hf.
-    rewrite Hf.
-    reflexivity.
-  Qed.
-
-  #[global] Instance arrayR_flip_mono X ty:
-    Proper (pointwise_relation nat (pointwise_relation X (flip (⊢))) ==> (=) ==> flip (⊢)) (parrayR ty).
-  Proof. solve_proper. Qed.
-  Hint Rewrite @skipn_0: syntactic.
-  Lemma generalize_arrayR_loopinv (i : nat) (p:ptr) {X : Type} (R : X → Rep) (ty : type) xs (Heq: i=0):
-    p |-> arrayR ty R xs
-    -|- (p  .[ty ! i]) |-> arrayR ty R (drop i xs).
-  Proof using.
-    intros.
-    apply: (observe_both (is_Some (size_of _ ty))) => Hsz.
-    subst.
-    autorewrite with syntactic.
-    reflexivity.
-  Qed.
-    
-  Lemma generalize_parrayR_loopinv (i : nat) (p:ptr) {X : Type} (R : nat -> X → Rep) (ty : type) xs (Heq: i=0):
-    p |-> parrayR ty R xs
-    -|- (p  .[ty ! i]) |-> parrayR ty (fun ii => R (i+ii)) (drop i xs).
-  Proof using.
-    intros.
-    apply: (observe_both (is_Some (size_of _ ty))) => Hsz.
-    subst.
-    autorewrite with syntactic.
-    reflexivity.
-  Qed.
-  
-  Lemma vectorbase_loopinv {T} ty base q (l: list T) (i:nat) (Heq: i=0):
-    VectorRbase ty q base (lengthN l) -|- (VectorRbase ty (q*Qp.inv (N_to_Qp (1+lengthN l))) base (lengthN l) ** 
-    ([∗ list] _ ∈ (drop i l),  VectorRbase ty (q*Qp.inv (N_to_Qp (1+lengthN l))) base (lengthN l))).
-  Proof using. Admitted.
-
-      Set Printing Coercions.
-    Lemma drop_S2: ∀ {A : Type} (l : list A) (n : nat),
-        (Z.of_nat n < lengthZ l)%Z→
-          exists x,  l !! n = Some x /\ drop n l = x :: drop (S n) l.
-    Proof using.
-      intros ? ? ? Hl.
-      unfold lengthN in Hl.
-      assert (n< length l)%nat as Hln by lia.
-      erewrite <- nth_error_Some in Hln.
-      pose proof (fun x => drop_S l x n).
-      rewrite <- lookup_nth_error in Hln.
-      destruct (l !! n); try congruence.
-      eexists; split; eauto.
-    Qed.
-
-       Ltac iExistsTac  foo:=match goal with
-                               |- environments.envs_entails _ (Exists (_:?T), _) => iExists ((ltac:(foo)):T)
-                             end.
-  Lemma parrayR_nil {T} (R : nat -> T -> Rep) ty: parrayR ty R [] -|- validR ** [| is_Some (size_of _ ty) |].
-  Proof using.
-    unfold parrayR. simpl.
-    apply: (observe_both (is_Some (size_of _ ty))) => Hsz.
-    change (Z.of_nat 0) with 0%Z.
-    autorewrite with syntactic.
-    rewrite _offsetR_sub_0; try assumption.
-    iSplit; work.
-  Qed.
-
-  Import linearity.
-
-  Lemma arrayR_cell {X} ty (R:X->Rep) xs i x iZ :
-    iZ = Z.of_nat i →	(** Ease [eapply] *)
-    xs !! i = Some x →	(** We have an [i]th element *)
-    arrayR ty R xs -|-
-           arrayR ty R (take i xs) **
-           _sub ty iZ |-> type_ptrR ty **
-           _sub ty iZ |-> R x **
-           _sub ty (iZ + 1) |-> arrayR ty R (drop (S i) xs).
-  Proof.
-    intros Hi Hl.
-    rewrite -{1}(take_drop_middle xs i _ Hl) arrayR_app arrayR_cons !_offsetR_sep.
-    f_equiv.
-    enough (length (take i xs) = i) as ->.
-    { subst. by rewrite _offsetR_sub_sub. }
-    { apply length_take_le.
-      apply lookup_lt_Some in Hl. lia. }
-  Qed.
-
-  Lemma parrayR_app {X} ty xs ys : forall (R:nat -> X->Rep),
-    parrayR ty R (xs ++ ys) -|- parrayR ty R xs ** .[ ty ! length xs ] |-> parrayR ty (fun ii => R (length xs +ii)) ys.
-  Proof.
-    induction xs => /=.
-    { unfold parrayR. intros.
-      apply: (observe_both (is_Some _)) => Hsz.
-      simpl.
-      change (Z.of_nat 0) with 0%Z.
-      repeat rewrite o_sub_0; auto.
-      repeat rewrite _offsetR_id.
-      iSplit; go. admit.
-      (*
-  _ : .[ ty ! Z.of_nat (length ys) ] |-> validR
-  --------------------------------------□
-  validR
-*)
-    }
-    { intros. repeat rewrite parrayR_cons.
-      by rewrite IHxs !_offsetR_sep !_offsetR_succ_sub Nat2Z.inj_succ -!assoc.
-    }
-  Admitted.
-  
-  Lemma parrayR_cell i {X} ty (R:nat -> X->Rep) xs x iZ :
-    iZ = Z.of_nat i →	(** Ease [eapply] *)
-    xs !! i = Some x →	(** We have an [i]th element *)
-    parrayR ty R xs -|-
-           parrayR ty R (take i xs) **
-           _sub ty iZ |-> type_ptrR ty **
-           _sub ty iZ |-> R i x **
-           _sub ty (iZ + 1) |-> parrayR ty (fun ii => R (S i+ii)) (drop (S i) xs).
-  Proof.
-    intros Hi Hl.
-    rewrite -{1}(take_drop_middle xs i _ Hl) parrayR_app parrayR_cons !_offsetR_sep.
-    f_equiv.
-    enough (length (take i xs) = i) as ->.
-    { subst. repeat setoid_rewrite _offsetR_sub_sub.
-      replace (i+0) with i by lia.
-      replace (Z.of_nat i + 0)%Z with (Z.of_nat i) by lia.
-      repeat setoid_rewrite Nat.add_succ_r.
-      iSplit; go.
-    }
-    { apply length_take_le.
-      apply lookup_lt_Some in Hl. lia. }
-  Qed.
-
-  Lemma parrayR_cell2 i {X} ty (R:nat -> X->Rep) xs:
-    (Z.of_nat i < Z.of_nat (length xs))%Z ->
-          exists x, 
-            xs !! i = Some x /\	(** We have an [i]th element *)
-    (parrayR ty R xs -|-
-           parrayR ty R (take i xs) **
-           _sub ty (Z.of_nat i) |-> type_ptrR ty **
-           _sub ty (Z.of_nat i) |-> R i x **
-           _sub ty ((Z.of_nat i) + 1) |-> parrayR ty (fun ii => R (S i+ii)) (drop (S i) xs)).
-  Proof using.
-    intros.
-    assert (i<length xs) as Hex by lia.
-    applyToSomeHyp @lookup_lt_is_Some_2.
-    hnf in autogenhyp.
-    forward_reason.
-    subst.
-    eexists; split; eauto.
-    apply parrayR_cell; auto.
-  Qed.
-
-  cpp.spec "monad::wait_for_promise(boost::fibers::promise<void>&)" as wait_for_promise with 
-          (
-            \arg{promise} "promise" (Vref promise)
-            \pre{(P:mpred) (g:gname)} promise |-> PromiseConsumerR g P
-            \post P ** promise |-> PromiseUnusableR).
-
-  Search arrayR equiv.
-  Lemma arrDecompose {T} (p:ptr) ltr (R: T -> Rep) (ty:type):
-    p |-> arrayR ty R ltr
-   -|- (valid_ptr (p .[ ty ! length ltr ])) ** [| is_Some (size_of CU ty) |] **
-     ( □ ([∗ list] k↦_ ∈ ltr, (type_ptr ty (p .[ ty ! k ])))) ∗
-      ([∗ list] k↦t ∈ ltr, p .[ ty ! k ] |-> R t).
-  Proof using.
-    rewrite arrayR_eq.
-    unfold arrayR_def.
-    rewrite arrR_eq.
-    unfold arrR_def.
-    repeat rewrite length_fmap.
-    repeat rewrite big_opL_fmap.
-    iSplit; go.
-    {
-      setoid_rewrite _offsetR_sep.
-      rewrite big_sepL_sep.
-      go.
-      repeat rewrite _at_big_sepL.
-      setoid_rewrite _at_offsetR.
-      go.
-      iClear "#".
-      iStopProof.
-      f_equiv.
-      go.
-    }
-    {
-      setoid_rewrite _offsetR_sep.
-      rewrite big_sepL_sep.
-      go.
-      repeat rewrite _at_big_sepL.
-      setoid_rewrite _at_offsetR.
-      go.
-       hideLhs.
-       rewrite big_sepL_proper; try go.
-       2:{ intros. iSplit. 2:{go.  evartacs.maximallyInstantiateLhsEvar. }  go. }
-       simpl.
-       unhideAllFromWork.
-       go.
-    }
-  Qed.
-
-  Lemma arrLearn (p:ptr) {T} ltr (R: T -> Rep) (ty:type):
-    p |-> arrayR ty R ltr
-   |-- (valid_ptr (p .[ ty ! length ltr ])) ** [| is_Some (size_of CU ty) |] **
-   ( □ ([∗ list] k↦_ ∈ ltr, (type_ptr ty (p .[ ty ! k ])))) **
-   p |-> arrayR ty R ltr.
-  Proof using.
-    iIntrosDestructs.
-    rewrite arrDecompose.
-    go.
-  Qed.
-
-  Lemma arrLearn2 (p:ptr) {T} ltr (R: T -> Rep) (ty:type):
-    p |-> arrayR ty R ltr
-   |-- valid_ptr p ** (valid_ptr (p .[ ty ! length ltr ])) ** [| is_Some (size_of CU ty) |] **
-   ( □ ([∗ list] k↦_ ∈ ltr, (type_ptr ty (p .[ ty ! k ])))) **
-   p |-> arrayR ty R ltr.
-  Proof using.
-    iIntrosDestructs.
-    rewrite arrDecompose.
-    go.
-    destruct ltr.
-    - go. autorewrite with syntactic. go.
-    -  simpl. autorewrite with syntactic. go.
-  Qed.
-
-  Lemma parrDecompose {T} (p:ptr) ltr (R: nat -> T -> Rep) (ty:type):
-    p |-> parrayR ty R ltr
-   -|- (valid_ptr (p .[ ty ! length ltr ])) ** [| is_Some (size_of CU ty) |] **
-     ( □ ([∗ list] k↦_ ∈ ltr, (type_ptr ty (p .[ ty ! k ])))) ∗
-      ([∗ list] k↦t ∈ ltr, p .[ ty ! k ] |-> R k t).
-  Proof using.
-    unfold parrayR.
-    repeat rewrite length_fmap.
-    repeat rewrite big_opL_fmap.
-    iSplit; go.
-    {
-      setoid_rewrite _offsetR_sep.
-      rewrite big_sepL_sep.
-      go.
-      repeat rewrite _at_big_sepL.
-      setoid_rewrite _at_offsetR.
-      go.
-      iClear "#".
-      iStopProof.
-      f_equiv.
-      go.
-    }
-    {
-      setoid_rewrite _offsetR_sep.
-      rewrite big_sepL_sep.
-      go.
-      repeat rewrite _at_big_sepL.
-      setoid_rewrite _at_offsetR.
-      go.
-       hideLhs.
-       rewrite big_sepL_proper; try go.
-       2:{ intros. iSplit. 2:{go.  evartacs.maximallyInstantiateLhsEvar. }  go. }
-       simpl.
-       unhideAllFromWork.
-       go.
-    }
-  Qed.
-
-  Lemma parrLearn (p:ptr) {T} ltr (R: nat -> T -> Rep) (ty:type):
-    p |-> parrayR ty R ltr
-   |-- (valid_ptr (p .[ ty ! length ltr ])) ** [| is_Some (size_of CU ty) |] **
-   ( □ ([∗ list] k↦_ ∈ ltr, (type_ptr ty (p .[ ty ! k ])))) **
-   p |-> parrayR ty R ltr.
-  Proof using.
-    iIntrosDestructs.
-    rewrite parrDecompose.
-    go.
-  Qed.
-
-  Lemma parrLearn2 (p:ptr) {T} ltr (R: nat -> T -> Rep) (ty:type):
-    p |-> parrayR ty R ltr
-   |-- valid_ptr p ** (valid_ptr (p .[ ty ! length ltr ])) ** [| is_Some (size_of CU ty) |] **
-   ( □ ([∗ list] k↦_ ∈ ltr, (type_ptr ty (p .[ ty ! k ])))) **
-   p |-> parrayR ty R ltr.
-  Proof using.
-    iIntrosDestructs.
-    rewrite parrDecompose.
-    go.
-    destruct ltr.
-    - go. autorewrite with syntactic. go.
-    -  simpl. autorewrite with syntactic. go.
-  Qed.
-  
-
-  Ltac hideP fullyHiddenPostcond :=
-      IPM.perm_left ltac:(fun L n =>
-                        match L with
-                        | HiddenPostCondition => hideFromWorkAs L fullyHiddenPostcond
-                        end
-                         ).
-
   cpp.spec (Nscoped 
-"monad::compute_senders(const monad::Block&, monad::fiber::PriorityPool&)::@0" (Nfunction function_qualifiers.N Ndtor []))  as cslamdestr inline.  
+              "monad::compute_senders(const monad::Block&, monad::fiber::PriorityPool&)::@0" (Nfunction function_qualifiers.N Ndtor []))  as cslamdestr inline.
+
+    Existing Instance learnArrUnsafe.
+  Existing Instance learnpArrUnsafe.
+
 Lemma prf: denoteModule module
              ** tvector_spec
              ** reset_promises
@@ -896,7 +221,7 @@ Proof using MODd.
                      ).
   rewrite (generalize_arrayR_loopinv ival (_global "monad::senders")); [| assumption].
   rewrite (generalize_arrayR_loopinv ival vectorbase); [| assumption].
-  rewrite (@vectorbase_loopinv _ _ _ _ _ ival); auto.
+  rewrite (vectorbase_loopinv _ _ _ _ ival); auto.
   IPM.perm_left ltac:(fun L n =>
                         match L with
                         | context[PromiseConsumerR] => hideFromWorkAs L pc
@@ -920,12 +245,12 @@ Proof using MODd.
     match goal with
       [H:_ |- _] => destruct H as [tri Htt]; destruct Htt as [Httl Httr]
     end.
-    rewrite Httr.
-    repeat rewrite -> arrayR_cons0.
+    repeat rewrite Httr.
+    repeat rewrite -> arrayR_cons.
     repeat rewrite -> parrayR_cons.
     go.
     autorewrite with syntactic.
-    repeat rewrite o_sub_sub.
+    progress repeat rewrite o_sub_sub.
     simpl.
     progress go.
     aggregateRepPieces a.
@@ -943,19 +268,16 @@ Proof using MODd.
     match goal with
         [ |-environments.envs_entails _ (?R -* _)] => iIntrosDestructs; iExists R
     end.
-    slauto.
-    iSplitL "".
+    go.
+    iSplitL ""%string.
     {
       unfold taskOpSpec.
       verify_spec'.
       slauto.
       iExists (N.of_nat ival). (* automate this using some Refine1 hint *)
       go.
-      Hint Rewrite nat_N_Z: syntactic.
       autorewrite with syntactic.
       slauto.
-      replace (ival + 0) with ival;[| lia].
-      go.
     }
     {
       slauto.
@@ -977,7 +299,6 @@ Proof using MODd.
     assert (ival=length(transactions block))  by lia.
     subst.
     go.
-    Hint Rewrite @drop_all: syntactic.
     autorewrite with syntactic.
     repeat rewrite arrayR_nil.
     repeat rewrite parrayR_nil.
@@ -1020,7 +341,6 @@ Proof using MODd.
       slauto.
       #[global] Instance : LearnEq2 PromiseConsumerR:= ltac:(solve_learnable).
       go.
-      Hint Rewrite Nat.add_0_r Z.add_0_r :syntactic.
       repeat rewrite o_sub_sub.
       autorewrite with syntactic.
       Set Printing Coercions.
@@ -1051,7 +371,6 @@ Proof using MODd.
       go.
       assert (ival=length(transactions block))  by lia.
       subst.
-    Hint Rewrite @firstn_all: syntactic.
       autorewrite with syntactic.
       go.
       repeat rewrite parrayR_nil. go.
