monadproofs/proofs/libspecs.v
@@ -1,2 +1,162 @@
+Require Import bedrock.auto.cpp.proof.
 
-Definition PriorityPool: Type. Admitted.
+Require Import monad.asts.exb.
+Require Import bedrock.auto.invariants.
+Require Import monad.proofs.evmopsem.
+Require Import monad.proofs.misc.
+
+Definition PriorityPool: Type. Proof using. Admitted.
+
+Section cp.
+  Import own.
+  Import frac.
+
+Context `{Sigma:cpp_logic} {CU: genv} {hh: HasOwn mpredI algebra.frac.fracR}. (* some standard assumptions about the c++ logic *)
+
+
+
+  (* defines how [c] is represented in memory as an object of class Chain *)
+  Definition PriorityPoolR (q: Qp) (c: PriorityPool): Rep. Proof using. Admitted.
+
+  Definition VectorRbase (cppType: type) (q:Qp) (base: ptr) (size: N): Rep.
+  Proof using.
+    (*Exists cap, 
+       _field "base" |-> ptrR q base
+       ** _field "size" |-> intR q size
+       ** _field "capacity" |-> intR q cap *)
+  Admitted.
+  
+ Definition VectorR {ElemType} (cppType: type) (elemRep: ElemType -> Rep) (q:Qp) (lt:list ElemType): Rep :=
+   Exists (base: ptr), VectorRbase cppType q base (lengthN lt)
+                         ** pureR (base |-> arrayR cppType elemRep lt).
+
+    (* set_value() passes the resource/assertion P to the one calling get_future->wait()*)
+  Definition PromiseR (g: gname) (P: mpred) : Rep. Proof using. Admitted.
+  Definition PromiseProducerR (g: gname) (P: mpred) : Rep. Proof using. Admitted.
+  Definition PromiseConsumerR (g: gname) (P: mpred) : Rep. Proof using. Admitted.
+  Definition PromiseUnusableR: Rep. Proof using. Admitted.
+
+  Lemma sharePromise g P:  PromiseR g P -|- PromiseProducerR g P **  PromiseConsumerR g P.
+  Proof using. Admitted.
+
+Context  {MODd : exb.module ⊧ CU}.
+(* Node::Node(Node*,int) *)
+  Definition promise_constructor_spec (this:ptr) :WpSpec mpredI val val :=
+    \pre{P:mpred} emp
+    \post Exists g:gname, this |->  PromiseR g P.
+
+  cpp.spec "boost::fibers::promise<void>::set_value()"  as set_value with
+     (fun (this:ptr) =>
+    \pre{(P:mpred) (g:gname)} this |-> PromiseProducerR g P
+    \pre P
+    \post emp).
+
+  cpp.spec
+    "std::vector<monad::Transaction, std::allocator<monad::Transaction>>::size() const"
+    as tvector_spec with
+      (fun (this:ptr) =>
+         \prepost{q base size} this |-> VectorRbase (Tnamed "::monad::Transaction")  q base size
+         \post[Vn size] (emp:mpred)
+      ).
+
+  Definition optionAddressR (q:Qp) (oaddr: option evm.address): Rep. Proof. Admitted.
+
+  cpp.spec "monad::wait_for_promise(boost::fibers::promise<void>&)" as wait_for_promise with 
+          (
+            \arg{promise} "promise" (Vref promise)
+            \pre{(P:mpred) (g:gname)} promise |-> PromiseConsumerR g P
+            \post P ** promise |-> PromiseUnusableR).
+
+  Lemma vectorbase_loopinv {T} ty base q (l: list T) (i:nat) (Heq: i=0):
+    VectorRbase ty q base (lengthN l) -|- (VectorRbase ty (q*Qp.inv (N_to_Qp (1+lengthN l))) base (lengthN l) ** 
+    ([∗ list] _ ∈ (drop i l),  VectorRbase ty (q*Qp.inv (N_to_Qp (1+lengthN l))) base (lengthN l))).
+  Proof using. Admitted.
+  Definition fork_task_namei:= Eval vm_compute in (firstEntryName (findBodyOfFnNamed2 exb.module (isFunctionNamed2 "fork_task"))).
+
+  Definition basee3 (n:name) :=
+    match n with
+    | Ninst (Nscoped (Nglobal (Nid scopename)) _) targs => scopename
+    | _ => ""%pstring
+    end.
+
+  Definition all_but_last {T:Type} (l: list T):= take (length l -1)%nat l. 
+  Definition fork_task_nameg (taskLamStructTy: core.name) :=
+    match fork_task_namei with
+    | Ninst (Nscoped (Nglobal (Nid scopename)) (Nfunction q (Nf base) argTypes)) templateArgs =>
+        let argTypes' := all_but_last argTypes ++  [Tref (Tqualified QC (Tnamed taskLamStructTy))] in
+        Ninst (Nscoped (Nglobal (Nid scopename)) (Nfunction q (Nf base) argTypes')) [Atype (Tnamed taskLamStructTy)]
+    | _ => Nunsupported "no match"
+    end.
+
+
+  Lemma fork_task_name_inst: exists ty, fork_task_nameg ty = fork_task_namei.
+  Proof using.
+    unfold fork_task_nameg. unfold fork_task_namei.
+    eexists. reflexivity.
+  Qed.
+
+  Definition taskOpName : atomic_name := Nfunction function_qualifiers.Nc (Nop OOCall) [].
+  
+  Definition taskOpSpec (lamStructName: core.name) (objOwnership: Rep) (taskPre: mpred):=
+    specify {| info_name :=  (Nscoped lamStructName taskOpName) ;
+              info_type := tMethod lamStructName QC "void" [] |}
+      (fun (this:ptr) =>
+         \prepost this |-> objOwnership
+         \pre taskPre
+         \post emp).
+  
+  Definition forkTaskSpec (lamStructName: core.name) : WpSpec mpredI val val :=
+    \arg{priority_poolp: ptr} "priority_pool" (Vref priority_poolp)
+    \prepost{priority_pool: PriorityPool} priority_poolp |-> PriorityPoolR 1 priority_pool
+    \arg{priority} "i" (Vint priority)  
+    \arg{task:ptr} "func" (Vref task)
+    \pre{objOwnership taskPre} taskOpSpec lamStructName objOwnership taskPre
+    \prepost task |-> objOwnership
+    \pre taskPre
+    \post emp.
+  
+  Lemma learnVUnsafe e t (r:e->Rep): LearnEq2 (VectorR t r).
+  Proof. solve_learnable. Qed.
+  Lemma learnVUnsafe2 e t: LearnEq3 (@VectorR e t).
+  Proof. solve_learnable. Qed.
+
+  Existing Instance learnVUnsafe2.
+  Lemma learnArrUnsafe e t: LearnEq2 (@arrayR _ _ _ e _ t).
+  Proof. solve_learnable. Qed.
+  Lemma learnpArrUnsafe e t: LearnEq2 (@parrayR _ _ _ _ e t).
+  Proof. solve_learnable. Qed.
+  
+  #[global] Instance learnVectorRbase: LearnEq4 VectorRbase:= ltac:(solve_learnable).
+  #[global] Instance learnPpool : LearnEq2 PriorityPoolR := ltac:(solve_learnable).
+
+
+  Definition vector_opg (cppType: type) (this:ptr): WpSpec mpredI val val :=
+    \arg{index} "index" (Vn index)
+    \prepost{qb base size} this |-> VectorRbase cppType qb base size
+    \require (index<size)%Z
+    \post [Vref (base ,, .[cppType!index])] emp.
+
+Opaque VectorR.
+
+       (* TODO: generalize over template arg *)
+  cpp.spec "std::optional<evmc::address>::operator=(std::optional<evmc::address>&&)" as opt_move_assign with
+    (fun (this:ptr) =>
+       \arg{other} "other" (Vptr other)
+       \pre{q oaddr} other |-> optionAddressR q oaddr
+       \pre{prev} this |-> optionAddressR 1 prev
+       \post [Vptr this] this |-> optionAddressR 1 oaddr **  other |-> optionAddressR q None
+    ).
+           
+  cpp.spec (Nscoped "std::optional<evmc::address>" (Nfunction function_qualifiers.N Ndtor [])) as destrop with
+      (fun (this:ptr) =>
+         \pre{oa} this |-> optionAddressR 1 oa
+           \post emp
+      ).
+  
+  #[global] Instance learnTrRbase2: LearnEq2 optionAddressR:= ltac:(solve_learnable).
+  #[global] Instance : LearnEq2 PromiseR := ltac:(solve_learnable).
+  #[global] Instance : LearnEq2 PromiseProducerR:= ltac:(solve_learnable).
+  
+End cp.
+
+
