monadproofs/proofs/misc.v
@@ -1,8 +1,40 @@
 Require Import QArith.
-Require Import bedrock.lang.cpp.
+Require Import bedrock.auto.cpp.proof.
+
 Require Import stdpp.gmap.
+Require Import bedrock.auto.cpp.tactics4.
 
 Import cQp_compat.
+Import linearity.
+Hint Rewrite @firstn_all: syntactic.
+Hint Rewrite Nat.add_0_r Z.add_0_r :syntactic.
+Hint Rewrite @drop_all: syntactic.
+Hint Rewrite nat_N_Z: syntactic.
+Hint Rewrite offset_ptr_sub_0 using (auto; apply has_size; exact _): syntactic.
+Hint Rewrite @skipn_0: syntactic.
+Ltac hideP fullyHiddenPostcond :=
+  IPM.perm_left ltac:(fun L n =>
+                        match L with
+                        | HiddenPostCondition => hideFromWorkAs L fullyHiddenPostcond
+                        end
+                     ).
+Ltac iExistsTac  foo:=match goal with
+                        |- environments.envs_entails _ (Exists (_:?T), _) => iExists ((ltac:(foo)):T)
+                      end.
+Ltac aggregateRepPieces base :=
+  repeat rewrite <- (_at_offsetR base);
+  repeat (IPM.perm_left ltac:(fun L n =>
+                                lazymatch L with
+                                | base |-> _ => iRevert n
+                                end
+    ));
+  repeat rewrite bi.wand_curry;
+  repeat rewrite <- _at_sep;
+  match goal with
+    [ |-environments.envs_entails _ (base |-> ?R -* _)] =>
+      iIntrosDestructs;
+      iExists R
+  end.
 
 #[local] Open Scope Z_scope.
 
@@ -13,4 +45,358 @@ Import cancelable_invariants.
 Definition storedAtGhostLoc  `{Sigma:cpp_logic} {CU: genv} (q: Q) (g: gname) (n: nat) : mpred.
   Admitted.
 
+
+Ltac slauto := go; try name_locals; tryif progress(try (ego; eagerUnifyU; go; fail); try (apply False_rect; try contradiction; try congruence; try nia; fail); try autorewrite with syntactic equiv iff slbwd in *; try rewrite left_id)
+  then slauto  else idtac.
   
+
+Section cp.
+  Context `{Sigma:cpp_logic} {CU: genv} {hh: HasOwn mpredI algebra.frac.fracR}. (* some standard assumptions about the c++ logic *)
+
+  Definition parrayR  {T:Type} ty (Rs : nat -> T -> Rep) (l: list T) : Rep :=
+  .[ ty ! length l ] |-> validR ** [| is_Some (size_of _ ty) |] **
+  (* ^ both of these are only relevant for empty arrays, otherwise, they are implied by the
+     following conjunct *)
+     [∗ list] i ↦ li ∈ l, .[ ty ! Z.of_nat i ] |-> (type_ptrR ty ** Rs i li).
+
+
+  Definition offsetR_only_fwd := ([BWD->] _offsetR_only_provable).
+  Hint Resolve offsetR_only_fwd: br_opacity.
+  Lemma parrayR_cons {T:Type} ty (R : nat -> T -> Rep) (x:T) (xs: list T) :
+    parrayR ty R (x :: xs) -|- type_ptrR ty ** (.[ ty ! 0 ] |-> (R 0 x)) ** .[ ty ! 1 ] |-> parrayR ty (fun n => R (S n)) xs.
+  Proof using.
+    unfold parrayR.
+    apply: (observe_both (is_Some (size_of _ ty))) => Hsz.
+    repeat rewrite !_offsetR_sub_0; auto.
+    repeat rewrite _offsetR_sep.
+    repeat rewrite _offsetR_big_sepL.
+    repeat rewrite _offsetR_succ_sub.
+    repeat setoid_rewrite  _offsetR_succ_sub.
+    simpl.
+    repeat rewrite Nat2Z.inj_succ.
+    repeat rewrite !_offsetR_sub_0; auto.
+    setoid_rewrite Nat2Z.inj_succ.
+    iSplit; work.
+  Qed.
+
+  Lemma arrDecompose {T} (p:ptr) ltr (R: T -> Rep) (ty:type):
+    p |-> arrayR ty R ltr
+   -|- (valid_ptr (p .[ ty ! length ltr ])) ** [| is_Some (size_of CU ty) |] **
+     ( □ ([∗ list] k↦_ ∈ ltr, (type_ptr ty (p .[ ty ! k ])))) ∗
+      ([∗ list] k↦t ∈ ltr, p .[ ty ! k ] |-> R t).
+  Proof using.
+    rewrite arrayR_eq.
+    unfold arrayR_def.
+    rewrite arrR_eq.
+    unfold arrR_def.
+    repeat rewrite length_fmap.
+    repeat rewrite big_opL_fmap.
+    iSplit; go.
+    {
+      setoid_rewrite _offsetR_sep.
+      rewrite big_sepL_sep.
+      go.
+      repeat rewrite _at_big_sepL.
+      setoid_rewrite _at_offsetR.
+      go.
+      iClear "#".
+      iStopProof.
+      f_equiv.
+      go.
+    }
+    {
+      setoid_rewrite _offsetR_sep.
+      rewrite big_sepL_sep.
+      go.
+      repeat rewrite _at_big_sepL.
+      setoid_rewrite _at_offsetR.
+      go.
+       hideLhs.
+       rewrite big_sepL_proper; try go.
+       2:{ intros. iSplit. 2:{go.  evartacs.maximallyInstantiateLhsEvar. }  go. }
+       simpl.
+       unhideAllFromWork.
+       go.
+    }
+  Qed.
+
+  Lemma arrLearn (p:ptr) {T} ltr (R: T -> Rep) (ty:type):
+    p |-> arrayR ty R ltr
+   |-- (valid_ptr (p .[ ty ! length ltr ])) ** [| is_Some (size_of CU ty) |] **
+   ( □ ([∗ list] k↦_ ∈ ltr, (type_ptr ty (p .[ ty ! k ])))) **
+   p |-> arrayR ty R ltr.
+  Proof using.
+    iIntrosDestructs.
+    rewrite arrDecompose.
+    go.
+  Qed.
+
+  Lemma arrLearn2 (p:ptr) {T} ltr (R: T -> Rep) (ty:type):
+    p |-> arrayR ty R ltr
+   |-- valid_ptr p ** (valid_ptr (p .[ ty ! length ltr ])) ** [| is_Some (size_of CU ty) |] **
+   ( □ ([∗ list] k↦_ ∈ ltr, (type_ptr ty (p .[ ty ! k ])))) **
+   p |-> arrayR ty R ltr.
+  Proof using.
+    iIntrosDestructs.
+    rewrite arrDecompose.
+    go.
+    destruct ltr.
+    - go. autorewrite with syntactic. go.
+    -  simpl. autorewrite with syntactic. go.
+  Qed.
+
+  Lemma parrDecompose {T} (p:ptr) ltr (R: nat -> T -> Rep) (ty:type):
+    p |-> parrayR ty R ltr
+   -|- (valid_ptr (p .[ ty ! length ltr ])) ** [| is_Some (size_of CU ty) |] **
+     ( □ ([∗ list] k↦_ ∈ ltr, (type_ptr ty (p .[ ty ! k ])))) ∗
+      ([∗ list] k↦t ∈ ltr, p .[ ty ! k ] |-> R k t).
+  Proof using.
+    unfold parrayR.
+    repeat rewrite length_fmap.
+    repeat rewrite big_opL_fmap.
+    iSplit; go.
+    {
+      setoid_rewrite _offsetR_sep.
+      rewrite big_sepL_sep.
+      go.
+      repeat rewrite _at_big_sepL.
+      setoid_rewrite _at_offsetR.
+      go.
+      iClear "#".
+      iStopProof.
+      f_equiv.
+      go.
+    }
+    {
+      setoid_rewrite _offsetR_sep.
+      rewrite big_sepL_sep.
+      go.
+      repeat rewrite _at_big_sepL.
+      setoid_rewrite _at_offsetR.
+      go.
+       hideLhs.
+       rewrite big_sepL_proper; try go.
+       2:{ intros. iSplit. 2:{go.  evartacs.maximallyInstantiateLhsEvar. }  go. }
+       simpl.
+       unhideAllFromWork.
+       go.
+    }
+  Qed.
+
+  Lemma parrLearn (p:ptr) {T} ltr (R: nat -> T -> Rep) (ty:type):
+    p |-> parrayR ty R ltr
+   |-- (valid_ptr (p .[ ty ! length ltr ])) ** [| is_Some (size_of CU ty) |] **
+   ( □ ([∗ list] k↦_ ∈ ltr, (type_ptr ty (p .[ ty ! k ])))) **
+   p |-> parrayR ty R ltr.
+  Proof using.
+    iIntrosDestructs.
+    rewrite parrDecompose.
+    go.
+  Qed.
+
+  Lemma parrLearn2 (p:ptr) {T} ltr (R: nat -> T -> Rep) (ty:type):
+    p |-> parrayR ty R ltr
+   |-- valid_ptr p ** (valid_ptr (p .[ ty ! length ltr ])) ** [| is_Some (size_of CU ty) |] **
+   ( □ ([∗ list] k↦_ ∈ ltr, (type_ptr ty (p .[ ty ! k ])))) **
+   p |-> parrayR ty R ltr.
+  Proof using.
+    iIntrosDestructs.
+    rewrite parrDecompose.
+    go.
+    destruct ltr.
+    - go. autorewrite with syntactic. go.
+    -  simpl. autorewrite with syntactic. go.
+  Qed.
+  
+
+  Lemma parrayR_app {X} ty xs ys : forall (R:nat -> X->Rep),
+    parrayR ty R (xs ++ ys) -|- parrayR ty R xs ** .[ ty ! length xs ] |-> parrayR ty (fun ii => R (length xs +ii)) ys.
+  Proof.
+    induction xs => /=.
+    { unfold parrayR. intros.
+      apply: (observe_both (is_Some _)) => Hsz.
+      simpl.
+      change (Z.of_nat 0) with 0%Z.
+      repeat rewrite o_sub_0; auto.
+      repeat rewrite _offsetR_id.
+      iSplit; go. admit.
+      (*
+  _ : .[ ty ! Z.of_nat (length ys) ] |-> validR
+  --------------------------------------□
+  validR
+*)
+    }
+    { intros. repeat rewrite parrayR_cons.
+      by rewrite IHxs !_offsetR_sep !_offsetR_succ_sub Nat2Z.inj_succ -!assoc.
+    }
+  Admitted.
+  
+  Lemma parrayR_cell i {X} ty (R:nat -> X->Rep) xs x iZ :
+    iZ = Z.of_nat i →	(** Ease [eapply] *)
+    xs !! i = Some x →	(** We have an [i]th element *)
+    parrayR ty R xs -|-
+           parrayR ty R (take i xs) **
+           _sub ty iZ |-> type_ptrR ty **
+           _sub ty iZ |-> R i x **
+           _sub ty (iZ + 1) |-> parrayR ty (fun ii => R (S i+ii)) (drop (S i) xs).
+  Proof.
+    intros Hi Hl.
+    rewrite -{1}(take_drop_middle xs i _ Hl) parrayR_app parrayR_cons !_offsetR_sep.
+    f_equiv.
+    enough (length (take i xs) = i) as ->.
+    { subst. repeat setoid_rewrite _offsetR_sub_sub.
+      replace (i+0) with i by lia.
+      replace (Z.of_nat i + 0)%Z with (Z.of_nat i) by lia.
+      repeat setoid_rewrite Nat.add_succ_r.
+      iSplit; go.
+    }
+    { apply length_take_le.
+      apply lookup_lt_Some in Hl. lia. }
+  Qed.
+
+  Lemma parrayR_cell2 i {X} ty (R:nat -> X->Rep) xs:
+    (Z.of_nat i < Z.of_nat (length xs))%Z ->
+          exists x, 
+            xs !! i = Some x /\	(** We have an [i]th element *)
+    (parrayR ty R xs -|-
+           parrayR ty R (take i xs) **
+           _sub ty (Z.of_nat i) |-> type_ptrR ty **
+           _sub ty (Z.of_nat i) |-> R i x **
+           _sub ty ((Z.of_nat i) + 1) |-> parrayR ty (fun ii => R (S i+ii)) (drop (S i) xs)).
+  Proof using.
+    intros.
+    assert (i<length xs) as Hex by lia.
+    applyToSomeHyp @lookup_lt_is_Some_2.
+    hnf in autogenhyp.
+    forward_reason.
+    subst.
+    eexists; split; eauto.
+    apply parrayR_cell; auto.
+  Qed.
+
+  Fixpoint isFunctionNamed2 (fname: ident) (n:name): bool :=
+    match n with
+    | Nglobal  (Nfunction _ (Nf i) _) => bool_decide (i=fname)
+    | Ninst nm _ => isFunctionNamed2 fname nm
+    | Nscoped _ (Nfunction _ (Nf i) _) => bool_decide (i=fname)
+    | _ => false
+    end.
+
+  Fixpoint containsDep (n:name): bool :=
+    match n with
+    | Ndependent _ => true
+    | Nglobal  (Nfunction _ (Nf i) _) => false
+    | Ninst nm _ => containsDep nm
+    | Nscoped nm (Nfunction _ (Nf i) _) => containsDep nm
+    | _ => false
+    end.
+  
+  Definition findBodyOfFnNamed2 module filter :=
+    List.filter (fun p => let '(nm, body):=p in filter nm) (NM.elements (symbols module)).
+
+
+  Definition firstEntryName (l :list (name * ObjValue)) :=
+    (List.nth 0 (map fst l) (Nunsupported "impossible")).
+  Lemma parrayR_sep {V} ty xs  : forall (A B : nat -> V -> Rep),
+    parrayR ty (fun i v => A i v ** B i v) xs -|-
+    parrayR ty (fun i v => A i v) xs **
+    parrayR ty (fun i v=> B i v) xs.
+  Proof.
+    elim: xs => [|x xs IH] /=; intros.
+    Transparent parrayR.
+    - unfold parrayR. simpl. iSplit; go.
+    - repeat rewrite parrayR_cons.  simpl.
+      rewrite {}IH. repeat rewrite _offsetR_sep.
+    all: iSplit; work.
+  Qed.
+
+  #[global] Instance parrayR_proper X ty:
+    Proper ((pointwise_relation nat (pointwise_relation X (≡))) ==> (=) ==> (≡)) (parrayR ty).
+  Proof.
+    unfold parrayR.
+    intros f g Hf xs y ?. subst. f_equiv.
+    f_equiv.
+    f_equiv.
+    hnf.
+    intros. hnf. intros.
+    hnf in Hf.
+    rewrite Hf.
+    reflexivity.
+  Qed.
+
+  #[global] Instance arrayR_mono X ty:
+    Proper (pointwise_relation nat (pointwise_relation X (⊢)) ==> (=) ==> (⊢)) (parrayR ty).
+  Proof.
+    unfold parrayR.
+    intros f g Hf xs y ?. subst. f_equiv.
+    f_equiv.
+    f_equiv.
+    hnf.
+    intros. hnf. intros.
+    hnf in Hf.
+    rewrite Hf.
+    reflexivity.
+  Qed.
+
+  #[global] Instance arrayR_flip_mono X ty:
+    Proper (pointwise_relation nat (pointwise_relation X (flip (⊢))) ==> (=) ==> flip (⊢)) (parrayR ty).
+  Proof. solve_proper. Qed.
+  Lemma generalize_arrayR_loopinv (i : nat) (p:ptr) {X : Type} (R : X → Rep) (ty : type) xs (Heq: i=0):
+    p |-> arrayR ty R xs
+    -|- (p  .[ty ! i]) |-> arrayR ty R (drop i xs).
+  Proof using.
+    intros.
+    apply: (observe_both (is_Some (size_of _ ty))) => Hsz.
+    subst.
+    autorewrite with syntactic.
+    reflexivity.
+  Qed.
+    
+  Lemma generalize_parrayR_loopinv (i : nat) (p:ptr) {X : Type} (R : nat -> X → Rep) (ty : type) xs (Heq: i=0):
+    p |-> parrayR ty R xs
+    -|- (p  .[ty ! i]) |-> parrayR ty (fun ii => R (i+ii)) (drop i xs).
+  Proof using.
+    intros.
+    apply: (observe_both (is_Some (size_of _ ty))) => Hsz.
+    subst.
+    autorewrite with syntactic.
+    reflexivity.
+  Qed.
+  
+  Lemma drop_S2: ∀ {A : Type} (l : list A) (n : nat),
+      (Z.of_nat n < lengthZ l)%Z→
+        exists x,  l !! n = Some x /\ drop n l = x :: drop (S n) l.
+  Proof using.
+    intros ? ? ? Hl.
+    unfold lengthN in Hl.
+    assert (n< length l)%nat as Hln by lia.
+    erewrite <- nth_error_Some in Hln.
+    pose proof (fun x => drop_S l x n).
+    rewrite <- lookup_nth_error in Hln.
+    destruct (l !! n); try congruence.
+    eexists; split; eauto.
+  Qed.
+
+  Lemma parrayR_nil {T} (R : nat -> T -> Rep) ty: parrayR ty R [] -|- validR ** [| is_Some (size_of _ ty) |].
+  Proof using.
+    unfold parrayR. simpl.
+    apply: (observe_both (is_Some (size_of _ ty))) => Hsz.
+    change (Z.of_nat 0) with 0%Z.
+    autorewrite with syntactic.
+    rewrite _offsetR_sub_0; try assumption.
+    iSplit; work.
+  Qed.
+  
+End cp.
+Opaque parrayR.
+Lemma cancelLstar {PROP:bi} {T} l (va vb : T -> PROP):
+  (forall id, id ∈ l -> va id |-- vb id) ->
+  ([∗ list] id ∈ l, va id) |-- ([∗ list] id ∈ l,vb id).
+Proof using.
+  intros He.
+  apply big_sepL_mono.
+  intros.
+  apply He.
+  eapply elem_of_list_lookup_2; eauto.
+Qed.
+Hint Opaque parrayR: br_opacity.
